continue working on simp

CustomSimpRw.lean
@@ -1,3 +1,4 @@
+import Batteries
 import Lean
 import Qq
 
@@ -9,11 +10,15 @@ open Qq
 
 Content
 (1) What simp & rw do on proof term level, and what is the difference?
-(2) Implementing basic `simp` & `rw` prototypes.
-(3) Unification -- rewriting a quantified equality.
-(4) Context & digging into quantifiers with simp.
+(2) Implementing `rw` using bare expressions.
+(3) Implementing `simp` using Qq.
+(4) Unification - rewriting a quantified equality.
 (5) Collecting tagged lemmas
 (6) Simplification procedures - building upon existing simp infrastructure
+
+Leave for another file
+* Options for `whnf`
+* Options for unification
 -/
 
 /-
@@ -25,15 +30,15 @@ that `simp only` rewrites as long as it can, while `rw` rewrites just once.
 The background reason is a fundamental differences between the terms
 proof produced.
 
-## rw
+## What `rw` does
 Let as look at an example proof using `rw`.
 -/
 
 theorem rw_example (a b : Nat) (f : Nat → Nat) (p : Nat → Prop)
-    (h_rw  : ∀ x : Nat, f x = x) (h_finish : p (a + b + a + b)) :
+    (h_eq  : ∀ x : Nat, f x = x) (h_finish : p (a + b + a + b)) :
     p (f a + f b + f a + f b) := by
-  rw [h_rw] -- rewrites two instances of `f a`
-  rw [h_rw] -- rewrites two instances of `f b`
+  rw [h_eq] -- rewrites two instances of `f a`
+  rw [h_eq] -- rewrites two instances of `f b`
   exact h_finish
 
 -- and print its proof term
@@ -42,28 +47,23 @@ theorem rw_example (a b : Nat) (f : Nat → Nat) (p : Nat → Prop)
 -- it should look similar to
 example : ∀ (a b : Nat) (f : Nat → Nat) (p : Nat → Prop),
   (∀ (x : Nat), f x = x) → p (a + b + a + b) → p (f a + f b + f a + f b) :=
-fun a b f p h_rw h_finish =>
+fun a b f p h_eq h_finish =>
   Eq.mpr (
-    congrArg (fun X => p (X + f b + X + f b)) (h_rw a : f a = a)
+    congrArg (fun X => p (X + f b + X + f b)) (h_eq a : f a = a)
     : p (f a + f b + f a + f b) = p (a + f b + a + f b)
   )
   (Eq.mpr (
-    congrArg (fun X => p (a + X + a + X)) (h_rw b : f b = b)
+    congrArg (fun X => p (a + X + a + X)) (h_eq b : f b = b)
     : p (a + f b + a + f b) = p (a + b + a + b)
   ) h_finish)
 
 -- You can see two main theorems used for each rewrite:
 #check congrArg -- digging into a subterm
-#check Eq.mpr -- finishing the proof
-
-#print Eq.rec
-#print Eq.ndrec
-#print Eq.mp
-#print cast
+#check Eq.mpr -- translate equality to implication
 
 /-
 Because of the theorems that `rw` is using, it first instantiates
-the hypothesis `h_rw`, and then replaces all the instances in the goal
+the hypothesis `h_eq`, and then replaces all the instances in the goal
 by a single call of `congrArg`.
 -/
 
@@ -87,7 +87,7 @@ def weirdNat : (fun t _ => t) Nat 8 := 4
 #check mkExpectedPropHint
 
 /-
-## simp
+## What `simp` does
 
 Simp doesn't do all its equal rewrites in one go.
 Instead, it recursively dives into the term, and when
@@ -97,33 +97,33 @@ updated, it directly uses
 #check congr
 
 theorem simp_example (a b c : Nat) (f : Nat → Nat) (p : Nat → Prop)
-    (h_rw  : ∀ x : Nat, f x = x) (h_finish : p (a + c + b + c + a + c)) :
+    (h_eq  : ∀ x : Nat, f x = x) (h_finish : p (a + c + b + c + a + c)) :
     p (f a + c + f b + c + f a + c) := by
-  simp only [h_rw]
+  simp only [h_eq]
   exact h_finish
 
 #print simp_example
 
 /-
-After some prettification, you could get the following term.
+After prettification, you could get the following proof term.
 -/
-theorem simp_example2 (a b c : Nat) (f : Nat → Nat) (p : Nat → Prop)
-    (h_rw  : ∀ x : Nat, f x = x) (h_finish : p (a + c + b + c + a + c)) :
+example (a b c : Nat) (f : Nat → Nat) (p : Nat → Prop)
+    (h_eq  : ∀ x : Nat, f x = x) (h_finish : p (a + c + b + c + a + c)) :
     p (f a + c + f b + c + f a + c) :=
   Eq.mpr
-  (congrArg (fun x => p (x + c))
+  (congrArg (fun X => p (X + c))
     (congr
-      (congrArg (fun x => (x + c + ·))
+      (congrArg (fun X => (X + c + ·))
         (congr
           (congrArg
-            (fun x => (x + c + ·)) (h_rw a : f a = a)
+            (fun X => (X + c + ·)) (h_eq a : f a = a)
             : (f a + c + ·) = (a + c + ·)
           )
-          (h_rw b : f b = b)
+          (h_eq b : f b = b)
           : f a + c + f b = a + c + b)
         : (f a + c + f b + c + ·) = (a + c + b + c + ·)
       )
-      (h_rw  a : f a = a)
+      (h_eq a : f a = a)
       : f a + c + f b + c + f a = a + c + b + c + a)
     : p (f a + c + f b + c + f a + c) = p (a + c + b + c + a + c)
   )
@@ -131,7 +131,7 @@ theorem simp_example2 (a b c : Nat) (f : Nat → Nat) (p : Nat → Prop)
 /-
 It is not as clean as with `rw`, but you can notice that
 * The expression is build gradually, not in one go.
-* We actually run `h_rw a` twice in the proof term, because
+* We actually run `h_eq a` twice in the proof term, because
   we are rewriting with it on two places, contrary to `rw`.
 -/
 
@@ -149,25 +149,299 @@ example (a b : Nat) (h_eq : a = b) (p : ∀ n : Nat, Fin n → Prop)
   exact h
 
 /-
-# (2) Implementing basic `simp` & `rw` prototypes.
-
-In the basic version, we will be only rewriting the a term
-with a single equality without quantifiers. The simp would
-process the term recursively but perhaps without repeated call
-to itself?
+Sure, in more basic cases, simp is able to rewrite
+inside binders because it uses special rules for that.
+Let's look at the following proof.
 -/
+theorem simp_example2 (a b : Nat) (p : Nat → Nat → Prop)
+    (h : a = b) (finish : ∀ x, p x b → p x b) : (∀ x, p x a → p x a) := by
+  simp only [h]
+  exact finish
 
-#check kabstract
-
--- TODO:
--- rw: implement variable extraction (or point to Lean implementation,
--- is it simple enough?) & full tactic replacing the goal
--- from that point on, we should only focus on a given term `t`,
--- with the intention to rewrite `t` to `s`, and give a proof of `t = s`.
--- And implement recursive simp of that form.
+-- If we print the proof term
+#print simp_example2
+-- we can see two special rules used
+#check implies_congr
+#check forall_congr
 
 /-
-# (3) Unification -- rewriting a quantified equality.
+# (2) Implementing `rw` using bare expressions.
+
+## Abstracting a variable
+
+In the basic version, we will be only rewriting a term
+with a single equality without quantifiers.
+
+Say we are rewriting `A = B` in some expression
+`e := ... A ... A ...`
+First, we want to locate all the `a`-s in the expression,
+and build a mapping
+`fun x => ... x ... x ...`
+
+This is called an abstraction, first we need to locate all `A`s in `e`,
+and replace them with a corresponding `bvar`.
+A `bvar` is a variable pointing to a quantifier with an index
+where quantifiers are indexed from the inner-most to the outer-most.
+To know the index for the `bvar`, we carry `offset`.
+-/
+def myAbstract (e a : Expr) (offset : Nat := 0) : MetaM Expr := do
+  if !e.hasLooseBVars then  -- we cannot rewrite a subterm containing a variable bound in `e`
+    if (← isDefEq e a) then  -- check if already `a` is already the root
+      return mkBVar offset  -- same as `Expr.bvar offset`
+  -- otherwise, we recurse
+  match e with
+  | .app f x         => return e.updateApp! (← myAbstract f a offset) (← myAbstract x a offset)
+  | .mdata _ b       => return e.updateMData! (← myAbstract b a offset) -- `b` = body
+  | .proj _ _ b      => return e.updateProj! (← myAbstract b a offset)
+  | .letE _ t v b _  =>
+    return e.updateLetE! (← myAbstract t a offset) -- diving under a binder -> increase offset
+      (← myAbstract v a offset) (← myAbstract b a (offset+1))
+  | .lam _ d b _     => return e.updateLambdaE! (← myAbstract d a offset) (← myAbstract b a (offset+1))
+  | .forallE _ d b _ => return e.updateForallE! (← myAbstract d a offset) (← myAbstract b a (offset+1))
+  | e                => return e
+
+-- lean implements this with a slightly more advanced but still readable
+#check kabstract
+
+-- Now, we can build the mapping
+def abstractToMapping (e a : Expr) : MetaM Expr := do
+  -- make sure that all previous mvar assignments were applied in `e`
+  -- this is necessary to recurse the term, not for `isDefEq`, so `a` doesn't need it
+  let e ← instantiateMVars e
+  let body ← myAbstract e a  -- replace `a` with a `bvar`
+  return mkLambda
+    `x -- name for the variable, due to `bvar`s, we don't have to care about collisions,
+    BinderInfo.default -- could be also e.g. `implicit` (braces instead of parentheses)
+    (← inferType a) -- type for the variable
+    body
+
+-- Let's test
+example (A : Nat) (h : -- some crazy expression containing various constructions
+    ∀ (y : Nat), (y = A) →
+    let z := A + y
+    y + A = (fun (x : Nat) => x + A - y) z -- no worry about the same name
+  ) : True := by
+  -- `run_tacq` is like `run_tac` but makes the context directly accessible
+  -- not useful for writing tactics but handy for testing
+  run_tacq
+    logInfo m!"Before: {h.ty}" -- Qq-type (compile-time)
+    let f ← abstractToMapping h.ty A
+    logInfo m!"After: {f}"
+  trivial
+
+/-
+## Decomposing equality
+-/
+/--
+`decomposeEq` takes a proof of equality `pf : a = b`, where `(a b : α : Sort u)`,
+and returns (u, α, a b)
+-/
+def decomposeEq (pf : Expr) : MetaM (Level × Expr × Expr × Expr) := do
+  let t ← inferType pf
+  let t ← whnf t -- helps to get `Eq` at the root, removing mdata, instantiating mvars...
+  match t with
+  | .app (.app (.app (.const ``Eq [u]) α) a) b =>
+    return (u, α, a, b)
+  | _ => throwError "given term {pf} : {t} is not a proof of equality"
+
+-- we also could have used `Expr.app3? ``Eq` but that doesn't give us the level
+#check Expr.app3?
+
+/-
+## Building proof term
+
+Now, we write a function that takes an equation
+a term `t := ... A ...`, and an equation `eq : A = B`,
+and returns a proof of `... B ... → ... A ...`.
+-/
+def proveRwImp (eq t : Expr) :
+  MetaM Expr := do
+  let (u, α, a, b) ← decomposeEq eq
+  -- find the abstract function
+  let f ← abstractToMapping t a
+  -- we also detect the sort level of t (usually Prop)
+  let tt ← inferType t
+  let v := (← inferType tt).sortLevel!
+  let rw_eq := mkApp6 -- build `@congrArg.{u,v} α tt a b f eq : f a = f b`
+    (mkConst ``congrArg [u,v])
+    α tt a b f eq
+  logInfo m!"rw_eq := {rw_eq}"
+  -- We know `f a = t` (definitionally)
+  -- Now let's calculate `f b` using famous "beta reduction".
+  let fb := f.beta #[b]
+  -- semantically it is the same as f.app b but the goal is not as pretty ;-)
+  -- try to uncomment the following line to see the difference:
+  -- let fb := f.app b
+  if !tt.isSort then -- why `t` must be a sort to build an implication?
+    throwError m!"Cannot convert equality between {tt} to an implication"
+  -- finally, let's build the implication
+  return mkApp3 -- build `Eq.mpr.{v-1} (f a) (f b) rw_eq`
+    (mkConst ``Eq.mpr [tt.sortLevel!])
+    t fb rw_eq
+
+#check congrArg
+#check Eq.mpr
+
+/-
+Let's test the function `proveRwImp`, and finish
+the goal rewrite inside `run_tacq` script
+-/
+example (a b : Nat) (h : a = b) : 2*a + b = 2*b + a := by
+  run_tacq goal =>
+    let t := q($a + 5 - $a)
+    -- try what happens with a non-prop term by uncommenting the next line
+    let imp ← proveRwImp h goal.ty
+    let imp_t ← inferType imp
+    -- test the result of `proveRwImp`
+    logInfo m!"imp : {imp_t}"
+    -- finish rewriting the goal
+    let mt := imp_t.bindingDomain!
+    logInfo m!"Build mvar of type {mt}"
+    let m ← mkFreshExprSyntheticOpaqueMVar mt
+    goal.mvarId!.assign (mkApp imp m)
+    replaceMainGoal [m.mvarId!]
+  -- check that we have successfully rewritten the main goal
+  rfl
+
+/-
+# (3) Implement `simp` using Qq
+
+For simp, we will utilize Qq to both showcase it, and to get some type safety.
+For start, we will not expect `simp` to automatically search for / apply theorems,
+we only provide it a finite list of fixed equalities it can use.
+
+We are not aiming at efficiency. Contrary to the standard `simp`
+which skips proving reflexivity, we will prove reflexivity at the atomic terms,
+and will propagate it upwards (just for for coding convenience).
+
+First, we define a structure capturing the result.
+-/
+/--
+The output of a simplification run on `a` of type `α : Sort u`
+is a proof `pf : a = b`. We need to store all of its typing
+information also to be able to specify its Qq-type.
+-/
+structure SimpResult {u : Level} {α : Q(Sort u)} (a : Q($α)) where
+  b : Q($α)
+  pf : Q($a = $b)
+
+-- Note that the library Simp also has a similar Result structure, both
+-- in basic library, and with Qq hints, we will not use that for now
+#check Simp.Result
+#check Simp.ResultQ
+
+/-
+Now, we prepare infrastructure for composing `SimpResult`s together.
+-/
+
+#check rfl
+/-- Builds a result for no rewrite -/
+def SimpResult.rfl {u : Level} {α : Q(Sort u)} (a : Q($α)) : SimpResult a := ⟨a, q(rfl)⟩
+
+def SimpResult.isRfl {u : Level} {α : Q(Sort u)} {a : Q($α)} (r : SimpResult a) :=
+  r.pf.isAppOfArity ``rfl 2
+
+#check Eq.trans
+/-- runs `Eq.trans` on `SimpResult`s -/
+def SimpResult.trans {u : Level} {α : Q(Sort u)} {a : Q($α)}
+    (r1 : SimpResult a) (r2 : SimpResult r1.b) : SimpResult a :=
+  let ⟨_,pf1⟩ := r1
+  let ⟨b2,pf2⟩ := r2
+  ⟨b2, q(Eq.trans $pf1 $pf2)⟩
+
+-- TODO: explain filling implicit variables
+-- TODO: tell about mkAppM
+
+-- TODO: explain there is a lot of work behind writing this
+
+#check congr
+/-- runs `congr` on `SimpResult`s -/
+def SimpResult.app {u v : Level} {α : Q(Sort u)} {β : Q(Sort v)}
+    {af : Q($α → $β)} {aArg : Q($α)}
+    (rf : @SimpResult _ q($α → $β) af) (rArg : SimpResult aArg) :
+    SimpResult q($af $aArg) :=
+  let ⟨bf, pff⟩ := rf
+  let ⟨bArg, pfArg⟩ := rArg
+  ⟨q($bf $bArg), q(@congr $α $β $af $bf $aArg $bArg $pff $pfArg)⟩
+
+#check implies_congr
+/-- runs `implies_congr` on `SimpResult`s -/
+def SimpResult.impl {u v : Level} {a1 : Q(Sort u)} {a2 : Q(Sort v)}
+    (r1 : @SimpResult _ q(Sort u) a1) (r2 : @SimpResult _ q(Sort v) a2) :
+    SimpResult (q($a1 → $a2)) :=
+  let ⟨b1, pf1⟩ := r1
+  let ⟨b2, pf2⟩ := r2
+  ⟨q($b1 → $b2), q(implies_congr $pf1 $pf2)⟩
+
+-- TODO: Notice we are sometimes in bare Expr
+
+#print forall_congr
+#check forall_congr
+def SimpResult.forall {u : Level} {α : Q(Sort u)}
+    (p q : Q($α → Prop)) (fv : Q($α)) (h : Q($p $fv = $q $fv))
+    (name : Name) (bi : BinderInfo) :
+    Q((∀ x, $p x) = (∀ x, $q x)) :=
+  have h : Q(∀ x, $p x = $q x) :=
+    mkLambda name bi α (h.abstract #[fv])
+  let res : Q((∀ x, $p x) = (∀ x, $q x)) :=
+    q(forall_congr $h)
+  -- we don't want to see the explicit applications `p a`, `p b`,
+  -- so we use `mkExpectedPropHint` to change the output type
+  -- to something definitionally equal.
+  have lhs : Q(Prop) := mkForall name bi α p.bindingBody!
+  have rhs : Q(Prop) := mkForall name bi α q.bindingBody!
+  mkExpectedPropHint res q($lhs = $rhs)
+
+/-
+TODO: explain better simpRec & simpBase
+
+To make it modular, we have
+* function `simpBase (...) a` that only tries to make a single rewrite step
+  of the root of `a` to `b` and build a proof of `a = b`. If the root doesn't,
+  simpllify, it just leaves `b` as `a`, and closes the proof with reflexivity.
+* recursive function `simpRec` which gets a specific
+  root-rewriting function as an argument, tries to apply
+  it anywhere inside the term, and returns the proof of equality in the same format.
+-/
+
+/--
+This is the main simple root-rewriting function.
+It gets a list of equalities `rules`, and tries to find a rule
+`rule : e = b` that exactly matches the given expression `e`.
+It doesn't dig inside `e`, and only tries to perform the step once.
+-/
+def simpBase (rules : List Expr) (u : Level) (α : Q(Sort u)) (a : Q($α)) :
+    MetaM (SimpResult a) := do
+  -- unfortunatelly, Qq-matching is not a friend with imperative constructions
+  -- such as `for .. do`, so we use a monadic alternative `List.findSomeM?`
+  let result? : Option (@SimpResult u α a)
+    ← rules.findSomeM? fun rule =>
+      have rule : Q(Prop) := rule
+      match rule with
+      | ~q($a = $b) =>
+        return (some ⟨b, rule⟩)
+      | _ => return none
+  return match result? with
+  | some result => result
+  | none => SimpResult.rfl a
+
+partial -- simplification could repeat indefinitely, `partial` skips termination check
+def simpRec (base : (u : Level) → (α : Q(Sort u)) → (a : Q($α)) →  MetaM (SimpResult a))
+  {u : Level} {α : Q(Sort u)} (a : Q($α)) : MetaM (SimpResult a) := do
+  -- Qq-matching doesn't work for highly abstract terms
+  -- TODO: whnf & match on
+  -- (f a)
+  -- (a → b)
+  -- ∀ x, p x
+  throwError "not finished"
+  -- TODO: simplify children
+  -- let prev : SimpResult := none.
+  -- match base e with
+  -- | none => prev
+  -- | some res =>
+
+/-
+# (4) Unification - rewriting a quantified equality.
 -/
 
 -- TODO:
@@ -178,20 +452,30 @@ to itself?
 -- * explain & run isDefEq
 
 /-
-# (4) Context & digging into quantifiers with simp.
--/
-
--- extensionality axiom
--- translating between bvars & fvars
-
-/-
 # (5) Collecting tagged lemmas
 -/
+
+-- TODO: look into it, understand, explain
+
+theorem cancel_around (x : Nat) : 1 + x - 1 = x := sorry
+
+attribute [simp] cancel_around
+-- TODO: look at gcongr example in mathlib
+#check registerSimpleScopedEnvExtension
+
+
+/-- Environment extension for "generalized congruence" (`gcongr`) lemmas. -/
+abbrev GCongrLemma := Nat
+
+initialize gcongrExt : SimpleScopedEnvExtension ((Name × Name × Array Bool) × GCongrLemma)
+    (Std.HashMap (Name × Name × Array Bool) (Array GCongrLemma)) ←
+  registerSimpleScopedEnvExtension {
+    addEntry := fun m (n, lem) => m.insert n ((m.getD n #[]).push lem)
+    initial := {}
+  }
 
 -- TODO
 
 /-
 # (6) Simplification procedures - building upon existing simp infrastructure
 -/
-
--- TODO
